Introducing old@ expressions. This includes: * Restrictions that labels aren't allowed to duplicate dominating labels. * Fixed bug: missing CanCall assumption in body of let-such-that expression. * Lifted previous implementation simplifcation (which seems no longer to be necessary), where all let-such-that were getting a heap argument. * Threading through heap-at expressions in various places, most notably in free-variable computations and in trigger computations.

Source/Dafny/Cloner.cs
@@ -345,7 +345,7 @@ namespace Microsoft.Dafny
 
       } else if (expr is OldExpr) {
         var e = (OldExpr)expr;
-        return new OldExpr(Tok(e.tok), CloneExpr(e.E));
+        return new OldExpr(Tok(e.tok), CloneExpr(e.E), e.At);
 
       } else if (expr is UnchangedExpr) {
         var e = (UnchangedExpr)expr;
