Source/Dafny/Triggers/QuantifiersCollector.cs
@@ -7,10 +7,10 @@ using System.Collections.ObjectModel;
 using System.Diagnostics.Contracts;
 
 namespace Microsoft.Dafny.Triggers {
-  internal class QuantifierCollector : TopDownVisitor<bool> {
+  internal class QuantifierCollector : TopDownVisitor<OldExpr/*?*/> {
     readonly ErrorReporter reporter;
     private readonly HashSet<Expression> quantifiers = new HashSet<Expression>();
-    internal readonly HashSet<Expression> exprsInOldContext = new HashSet<Expression>();
+    internal readonly Dictionary<Expression, HashSet<OldExpr>> exprsInOldContext = new Dictionary<Expression, HashSet<OldExpr>>();
     internal readonly List<QuantifiersCollection> quantifierCollections = new List<QuantifiersCollection>();
 
     public QuantifierCollector(ErrorReporter reporter) {
@@ -18,7 +18,7 @@ namespace Microsoft.Dafny.Triggers {
       this.reporter = reporter;
     }
 
-    protected override bool VisitOneExpr(Expression expr, ref bool inOldContext) {
+    protected override bool VisitOneExpr(Expression expr, ref OldExpr/*?*/ enclosingOldContext) {
       var e = expr as ComprehensionExpr;
 
       // only consider quantifiers that are not empty (Bound.Vars.Count > 0)
@@ -40,9 +40,17 @@ namespace Microsoft.Dafny.Triggers {
       }
 
       if (expr is OldExpr) {
-        inOldContext = true;
-      } else if (inOldContext) { // FIXME be more restrctive on the type of stuff that we annotate
-        exprsInOldContext.Add(expr);
+        enclosingOldContext = (OldExpr)expr;
+      } else if (enclosingOldContext != null) { // FIXME be more restrctive on the type of stuff that we annotate
+        // Add the association (expr, oldContext) to exprsInOldContext. However, due to chaining expressions,
+        // expr may already be a key in exprsInOldContext.
+        HashSet<OldExpr> prevValue;
+        if (exprsInOldContext.TryGetValue(expr, out prevValue)) {
+          prevValue.Add(enclosingOldContext);
+        } else {
+          var single = new HashSet<OldExpr>() { enclosingOldContext };
+          exprsInOldContext.Add(expr, single);
+        }
       }
 
       bool shouldContinue = true;
@@ -51,7 +59,7 @@ namespace Microsoft.Dafny.Triggers {
         if (le.LHSs.All(p => p.Var != null) && le.Exact) {
           // inline this let-expr and visit the resulting expression rather than continuing this visitor
           var newExpr = Translator.InlineLet(le);
-          this.Visit(newExpr, inOldContext);
+          this.Visit(newExpr, enclosingOldContext);
           shouldContinue = false;
         }
       }
@@ -59,7 +67,7 @@ namespace Microsoft.Dafny.Triggers {
       return shouldContinue;
     }
 
-    protected override bool VisitOneStmt(Statement stmt, ref bool st) {
+    protected override bool VisitOneStmt(Statement stmt, ref OldExpr/*?*/ st) {
       if (stmt is ForallStmt) {
         ForallStmt s = (ForallStmt)stmt;
         if (s.ForallExpressions != null) {
