Test/dafny0/LabelsOldAt.dfy
@@ -1,0 +1,57 @@
+// RUN: %dafny /print:"%t.print" /dprint:"%t.dprint" "%s" > "%t"
+// RUN: %diff "%s.expect" "%t"
+
+class C {
+  var x: int
+
+  method M()
+    requires x == 6
+    modifies this
+  {
+    x := 10;
+    label 00:
+    label 01:
+    x := x + 1;
+    label 2:
+    {
+      label 0_2:
+      x := x + 1;
+      label 3:
+      assert true;
+    }
+    label 0003:
+    x := x + 1;
+    label four:
+    x := x + 1;
+    assert old(x) == 6;
+
+    assert old@00(x) == old@01(x) == 10;
+    assert old@2(x) == old@0_2(x) == 11;
+    assert old@3(x) == 12 == old@0003(x);
+    assert old@four(x) == 13;
+    assert x == 14;
+    assert x == old(x);  // error: (just to check that not everything is provable)
+  }
+
+  method Lets(i: int, whoKnows: bool) returns (o: int)
+    requires x == i == 10
+    modifies this
+    ensures 4*o == 24
+  {
+    x := x + 3;
+    label 7:  // x == 13
+    x := x + 5;
+    o := i - 4;
+    assert o == var six :| six == 6; six;
+    label L8:  // x == 18
+    x := 2;
+    ghost var k :| k == x + old(x) + old@7(x) + old@L8(x);  // assign such that
+    assert k == 2 + 10 + 13 + 18;
+    ghost var m :=
+      var k :| k == x + old(x) + old@7(x) + old@L8(x); k;  // let such that
+    assert m == 2 + 10 + 13 + 18;
+    assert o == var six :| six == 6; six;
+    assert o == 18 - var twelve :| twelve == 12; twelve;
+    assert whoKnows;  // error: no evidence that it holds (or doesn't hold)
+  }
+}
